analysis/basic/interference_bound_edf.v
@@ -135,21 +135,19 @@ Module InterferenceBoundEDF.
     Hypothesis H_completed_jobs_dont_execute:
       completed_jobs_dont_execute job_cost sched.
 
-    (* Also assume that jobs do not execute in parallel and that
-       there exists at least one processor. *)
-    Hypothesis H_no_parallelism:
-      jobs_dont_execute_in_parallel sched.
-    Hypothesis H_at_least_one_cpu :
-      num_cpus > 0.
+    (* Also assume that jobs are sequential and that there exists at
+       least one processor. *)
+    Hypothesis H_sequential_jobs: sequential_jobs sched.
+    Hypothesis H_at_least_one_cpu: num_cpus > 0.
 
     (* Consider a task set ts where all jobs come from the task set
-       and tasks have valid parameters and restricted deadlines. *)
+       and tasks have valid parameters and constrained deadlines. *)
     Variable ts: taskset_of sporadic_task.
     Hypothesis all_jobs_from_taskset:
       forall (j: JobIn arr_seq), job_task j \in ts.
     Hypothesis H_valid_task_parameters:
       valid_sporadic_taskset task_cost task_period task_deadline ts.
-    Hypothesis H_restricted_deadlines:
+    Hypothesis H_constrained_deadlines:
       forall tsk, tsk \in ts -> task_deadline tsk <= task_period tsk.
 
     Let no_deadline_is_missed_by_tsk (tsk: sporadic_task) :=
@@ -736,7 +734,7 @@ Module InterferenceBoundEDF.
               apply leq_trans with (n := a_fst + p_k).
               {
                 by rewrite leq_add2l; apply leq_trans with (n := D_k);
-                  [by apply H_R_k_le_deadline | by apply H_restricted_deadlines].
+                  [by apply H_R_k_le_deadline | by apply H_constrained_deadlines].
               }
             
               (* Since jobs are sporadic, we know that the first job arrives
