analysis/jitter/bertogna_edf_theory.v
@@ -52,22 +52,20 @@ Module ResponseTimeAnalysisEDFJitter.
     Hypothesis H_completed_jobs_dont_execute:
       completed_jobs_dont_execute job_cost sched.
 
-    (* Also assume that jobs do not execute in parallel and that
-       there exists at least one processor. *)
-    Hypothesis H_no_parallelism:
-      jobs_dont_execute_in_parallel sched.
-    Hypothesis H_at_least_one_cpu :
-      num_cpus > 0.
+    (* Also assume that jobs are sequential and that there exists
+       at least one processor. *)
+    Hypothesis H_sequential_jobs: sequential_jobs sched.
+    Hypothesis H_at_least_one_cpu: num_cpus > 0.
 
     (* Assume that we have a task set ts, such that all jobs come
        from the task set, and all tasks have valid parameters and
-       restricted deadlines. *)
+       constrained deadlines. *)
     Variable ts: taskset_of sporadic_task.
     Hypothesis H_all_jobs_from_taskset:
       forall (j: JobIn arr_seq), job_task j \in ts.
     Hypothesis H_valid_task_parameters:
       valid_sporadic_taskset task_cost task_period task_deadline ts.
-    Hypothesis H_restricted_deadlines:
+    Hypothesis H_constrained_deadlines:
       forall tsk, tsk \in ts -> task_deadline tsk <= task_period tsk.
 
     Let no_deadline_is_missed_by_tsk (tsk: sporadic_task) :=
@@ -184,7 +182,7 @@ Module ResponseTimeAnalysisEDFJitter.
           rename H_all_previous_jobs_completed_on_time into BEFOREok,
                  H_valid_job_parameters into PARAMS,
                  H_valid_task_parameters into TASK_PARAMS,
-                 H_restricted_deadlines into RESTR,
+                 H_constrained_deadlines into RESTR,
                  H_tasks_miss_no_deadlines into NOMISS.
           unfold x, task_interference, valid_sporadic_job_with_jitter, valid_sporadic_job in *.
           have INts := bertogna_edf_tsk_other_in_ts.
@@ -296,7 +294,7 @@ Module ResponseTimeAnalysisEDFJitter.
                  H_all_previous_jobs_completed_on_time into BEFOREok,
                  H_tasks_miss_no_deadlines into NOMISS,
                  H_rt_bounds_contains_all_tasks into UNZIP,
-                 H_restricted_deadlines into RESTR,
+                 H_constrained_deadlines into RESTR,
                  H_work_conserving into WORK.
           unfold valid_sporadic_job_with_jitter, valid_sporadic_job in *.
           move => t /andP [LEt LTt] BACK.
@@ -348,7 +346,7 @@ Module ResponseTimeAnalysisEDFJitter.
                  H_tsk_R_in_rt_bounds into INbounds,
                  H_all_previous_jobs_completed_on_time into BEFOREok,
                  H_tasks_miss_no_deadlines into NOMISS,
-                 H_restricted_deadlines into RESTR.
+                 H_constrained_deadlines into RESTR.
           unfold sporadic_task_model, valid_sporadic_job_with_jitter, valid_sporadic_job in *.
           unfold x, X, total_interference, task_interference.
           rewrite -big_mkcond -exchange_big big_distrl /=.
@@ -388,7 +386,7 @@ Module ResponseTimeAnalysisEDFJitter.
                  H_tsk_R_in_rt_bounds into INbounds,
                  H_all_previous_jobs_completed_on_time into BEFOREok,
                  H_tasks_miss_no_deadlines into NOMISS,
-                 H_restricted_deadlines into RESTR.
+                 H_constrained_deadlines into RESTR.
           unfold sporadic_task_model in *.
           intros delta HAS.
           set some_interference_A := fun t =>
