analysis/jitter/interference_bound_edf.v
@@ -138,21 +138,19 @@ Module InterferenceBoundEDFJitter.
     Hypothesis H_completed_jobs_dont_execute:
       completed_jobs_dont_execute job_cost sched.
 
-    (* Also assume that jobs do not execute in parallel and that
-       there exists at least one processor. *)
-    Hypothesis H_no_parallelism:
-      jobs_dont_execute_in_parallel sched.
-    Hypothesis H_at_least_one_cpu :
-      num_cpus > 0.
+    (* Also assume that jobs are sequential and that there exists
+       at least one processor. *)
+    Hypothesis H_sequential_jobs: sequential_jobs sched.
+    Hypothesis H_at_least_one_cpu: num_cpus > 0.
 
     (* Assume that we have a task set where all tasks have valid
-       parameters and restricted deadlines. *)
+       parameters and constrained deadlines. *)
     Variable ts: taskset_of sporadic_task.
     Hypothesis all_jobs_from_taskset:
       forall (j: JobIn arr_seq), job_task j \in ts.
     Hypothesis H_valid_task_parameters:
       valid_sporadic_taskset task_cost task_period task_deadline ts.
-    Hypothesis H_restricted_deadlines:
+    Hypothesis H_constrained_deadlines:
       forall tsk, tsk \in ts -> task_deadline tsk <= task_period tsk.
 
     Let no_deadline_is_missed_by_tsk (tsk: sporadic_task) :=
@@ -821,7 +819,7 @@ Module InterferenceBoundEDFJitter.
               {
                 apply leq_trans with (n := job_arrival j_fst + D_k);
                   first by rewrite -addnA leq_add2l.
-                by rewrite leq_add2l; apply H_restricted_deadlines. 
+                by rewrite leq_add2l; apply H_constrained_deadlines. 
               }
             
               (* Since jobs are sporadic, we know that the first job arrives
