analysis/parallel/bertogna_edf_theory.v
@@ -54,13 +54,13 @@ Module ResponseTimeAnalysisEDF.
 
     (* Assume that we have a task set ts such that all jobs come from
        the task set, and all tasks have valid parameters and
-       restricted deadlines. *)
+       constrained deadlines. *)
     Variable ts: taskset_of sporadic_task.
     Hypothesis H_all_jobs_from_taskset:
       forall (j: JobIn arr_seq), job_task j \in ts.
     Hypothesis H_valid_task_parameters:
       valid_sporadic_taskset task_cost task_period task_deadline ts.
-    Hypothesis H_restricted_deadlines:
+    Hypothesis H_constrained_deadlines:
       forall tsk, tsk \in ts -> task_deadline tsk <= task_period tsk.
 
     Let no_deadline_is_missed_by_tsk (tsk: sporadic_task) :=
@@ -174,7 +174,7 @@ Module ResponseTimeAnalysisEDF.
           rename H_all_previous_jobs_completed_on_time into BEFOREok,
                  H_valid_job_parameters into PARAMS,
                  H_valid_task_parameters into TASK_PARAMS,
-                 H_restricted_deadlines into RESTR,
+                 H_constrained_deadlines into RESTR,
                  H_tasks_miss_no_deadlines into NOMISS.
           unfold x, task_interference.
           have INts := bertogna_edf_tsk_other_in_ts.
@@ -267,7 +267,7 @@ Module ResponseTimeAnalysisEDF.
                H_all_previous_jobs_completed_on_time into BEFOREok,
                H_tasks_miss_no_deadlines into NOMISS,
                H_rt_bounds_contains_all_tasks into UNZIP,
-               H_restricted_deadlines into RESTR.
+               H_constrained_deadlines into RESTR.
         unfold sporadic_task_model in *.
         unfold x, X, total_interference, task_interference.
         rewrite -big_mkcond -exchange_big big_distrl /=.
