model/basic/platform_fp.v
@@ -50,9 +50,8 @@ Module PlatformFP.
       Hypothesis H_all_jobs_from_taskset:
         forall (j: JobIn arr_seq), job_task j \in ts.
 
-      (* Suppose that a single job does not execute in parallel, ...*)
-      Hypothesis H_no_parallelism:
-        jobs_dont_execute_in_parallel sched.
+      (* Suppose that jobs are sequential, ...*)
+      Hypothesis H_sequential_jobs: sequential_jobs sched.
       (* ... jobs must arrive to execute, ... *)
       Hypothesis H_completed_jobs_dont_execute:
         completed_jobs_dont_execute job_cost sched.
@@ -177,7 +176,7 @@ Module PlatformFP.
         count (scheduled_task_with_higher_eq_priority tsk) ts = num_cpus.
       Proof.
         rename H_all_jobs_from_taskset into FROMTS,
-               H_no_parallelism into SEQUENTIAL,
+               H_sequential_jobs into SEQUENTIAL,
                H_work_conserving into WORK,
                H_enforces_JLDP_policy into PRIO,
                H_j_backlogged into BACK,
@@ -195,7 +194,7 @@ Module PlatformFP.
                task_precedence_constraints, completed_jobs_dont_execute,
                sporadic_task_model, is_valid_sporadic_task,
                jobs_of_same_task_dont_execute_in_parallel,
-               jobs_dont_execute_in_parallel,
+               sequential_jobs,
                can_interfere_with_tsk in *.
         have UNIQ := platform_fp_no_multiple_jobs_of_interfering_tasks.
         have UNIQ' := platform_fp_no_multiple_jobs_of_tsk. 
